LeanAideTools/ClashExample.lean
@@ -1,0 +1,62 @@
+import LeanAideTools.InstanceClash
+import LeanAideTools.AsyncMode
+/-!
+Example usage
+-/
+
+instance collapseInst : HAdd String String String where
+  hAdd := String.append
+
+def collapse (a b: String): String :=
+  @HAdd.hAdd String String String collapseInst a b
+
+instance collapseInst' : HAdd String String String where
+  hAdd := fun a b => a ++ " " ++ b
+
+def collapse' (a b: String): String :=
+  @HAdd.hAdd String String String collapseInst' a b
+
+
+/--
+error: instances clash: `collapseInst'` and `collapseInst` are instances of the same typeclass `HAdd String String
+  String` with different instances.
+-/
+#guard_msgs in
+example (a b  : String) : collapse' a b = collapse a b := by
+  unfold collapse collapse'
+  check_clashes
+
+/--
+warning: instances clash: `collapseInst'` and `collapseInst` are instances of the same typeclass `HAdd String String
+  String` with different instances.
+---
+error: unsolved goals
+a b : String
+⊢ a + b = a + b
+-/
+#guard_msgs in
+example (a b  : String) : collapse' a b = collapse a b := by
+  unfold collapse collapse'
+  warn_clashes
+
+example (a b  : String) : collapse' a b = collapse a b := by
+  unfold collapse collapse'
+  try check_clashes
+  sorry
+
+example (a b  : String) : collapse' a b = collapse a b := by
+  unfold collapse collapse'
+  warn_clashes
+  sorry
+
+/--
+error: Error in fail tactic check_clashes: instances clash: `collapseInst'` and `collapseInst` are instances of the same typeclass `HAdd
+  String String String` with different instances.
+---
+error: unsolved goals
+a b : String
+⊢ a + b = a + b
+-/
+#guard_msgs in
+example (a b  : String) : collapse' a b = collapse a b := byy
+  unfold collapse collapse'
